More work on erc20

CoqOfRust/ink/update_after_translation.py
@@ -777,33 +777,6 @@ Require CoqOfRust.ink.ink_env.
 (* @TODO Require CoqOfRust.ink.ink. *)
 
 (** @TODO [erc20] dependencies which are WIP *)
-Module ink_env.
-  Module types.
-
-    Parameter DefaultEnvironment : Set.
-    
-    Module Environment.
-      Parameter AccountId : Set.
-      Parameter Balance : Set.
-      Parameter Hash : Set.
-      Parameter Timestamp : Set.
-      Parameter BlockNumber : Set.
-      Parameter ChainExtension : Set.
-      Parameter MAX_EVENT_TOPICS : usize.
-    End Environment.
-  End types.
-  
-  Module contract.
-    Module ContractEnv.
-      Unset Primitive Projections.
-      Class Trait (Self : Set) : Type := {
-          Env : Set
-        }.
-      Global Set Primitive Projections.
-    End ContractEnv.
-
-  End contract.
-End ink_env.
 
 Module ink.
   Module codegen.
@@ -888,6 +861,29 @@ End ink.
   End Erc20.
   Definition Erc20 : Set := @Erc20.t.
 """,
+        content,
+    )
+
+    content = sub_exactly_once(
+        """    Definition Env : Set := ink_env.types.DefaultEnvironment.""",
+        """    Definition Env : Set := ink_env.types.DefaultEnvironment.
+
+    Global Instance Impl_Environment_for_Env : ink_env.types.Environment.Trait Env. Admitted.
+    Global Hint Resolve Impl_Environment_for_Env : core.""",
+        content,
+    )
+
+    content = sub_exactly_once(
+        """    Global Instance I : ink_env.contract.ContractEnv.Trait Self := {
+      ink_env.contract.ContractEnv.Env := Env;
+    }.""",
+        """    #[refine]
+    Global Instance I : ink_env.contract.ContractEnv.Trait Self := {
+      ink_env.contract.ContractEnv.Env := Env;
+    }.
+    eauto.
+    Defined.
+    Global Hint Resolve I : core.""",
         content,
     )
 
